Implement priority

Treap.dfy
@@ -1,36 +1,111 @@
 include "TreapNode.dfy"
 
 class Treap {
-  var root: TreapNode?
-  var prioritySet: set<int> //Keeps track of what priority was used.
-
-  constructor () 
-  ensures Valid()
-  {
-    this.root := null;
-  }
+  /** ---- Ghost Information ---- */
+  ghost var Values: set<int>
+  ghost var Priorities: set<int>
+  ghost var Repr: set<object>
 
   ghost predicate Valid()
-    reads this, root, if root != null then root.repr else {}
+    reads this, Repr
+    ensures Valid() ==> this in Repr
   {
-    root != null ==> root.Valid()
+    // This class must be inside set Repr
+    && this in Repr
+    // Make sure everything is empty if the root is not set
+    && (root == null ==> Values == {} && Priorities == {})
+    // This tree must hold the same information with the root 
+    && (root != null ==> 
+        && root in Repr 
+        && root.Repr <= Repr
+        && this !in root.Repr
+        && root.Valid() && root.ValidHeap()
+        && Values == root.Values
+        && Priorities == root.Priorities)
   }
 
+  /** ---- Class Attributes ---- */
+  var root: TreapNode?
 
-  method Build(values: array<int>) {}
-  method Insert(value: int) 
-    modifies this;
-    modifies if this.root != null then this.root.repr else {}
-    requires this.root != null ==> this.root.Valid()
-    // requires this.root != null ==> this.root in this.root.repr
-    // ensures this.root != null ==> this.root.Valid()
+  constructor () 
+    ensures Valid() && fresh(Repr)
+    ensures Values == {} && Priorities == {}
   {
-    var priority := value * 123 % 1000;
-    var node := new TreapNode(value, priority);
-    if (this.root != null) {
-      this.root.insertNode(node);
+    this.root := null;
+    Repr := {this};
+    Values := {};
+    Priorities := {};
+  }
+
+  /** ----- Class Methods ------ */
+  method Build(values: array<int>) {}
+
+  method Insert(val: int)
+    requires Valid()
+    modifies Repr;
+    ensures Valid() && fresh(Repr - old(Repr))
+  {
+    var priority: int := val * 123 % 1000; // TODO: define a proper priority
+    if (root == null) {
+      root := new TreapNode(val, priority);
+      Repr := root.Repr + {this};
+      Values := root.Values;
+      Priorities := root.Priorities;
+    }
+
+    // TODO: assert priority
+  }
+
+  static method InsertHelper(val: int, priority: int, node: TreapNode) returns (head: TreapNode?)
+    requires node.Valid() && node.ValidHeap()
+    modifies node.Repr
+    ensures head != null ==> head.Valid() && head.ValidHeap()
+    ensures node.Valid() && node.ValidHeap()
+    decreases node.Repr
+  {
+    head := null;
+    if (node.value == val) {
+      head := node;
     } else {
-      this.root := node;
+      if (val < node.value) {
+        if (node.left == null && priority > node.priority) {
+          var abc := new TreapNode(val, priority);
+          node.left := abc;
+          node.Repr := {node} + node.left.Repr + if node.right != null then node.right.Repr else {};
+          node.Values := {node.value} + node.left.Values + if node.right != null then node.right.Values else {};
+          node.Priorities := {node.priority} + node.left.Priorities + if node.right != null then node.right.Priorities else {};
+          head := node;
+          if (node.left.priority > node.priority) {
+            head := RotateRight(node);
+          }
+          assert node.Valid() && node.ValidHeap();
+        } else if (node.left != null) {
+          // var leftSide := InsertHelper(val, priority, node.left);
+          // if (leftSide != null) {
+          //   node.Repr := {node} + leftSide.Repr + if node.right != null then node.right.Repr else {};
+          //   node.Values := {node.value} + leftSide.Values + if node.right != null then node.right.Values else {};
+          //   node.Priorities := {node.priority} + leftSide.Priorities + if node.right != null then node.right.Priorities else {};
+          //   node.left := leftSide;
+          //   head := node;
+          //   if (node.left.priority > node.priority) {
+          //     head := RotateRight(node);
+          //   }
+          // }
+        } 
+      } else {
+        if (node.right == null && priority > node.priority) {
+          var abc := new TreapNode(val, priority);
+          node.right := abc;
+          node.Repr := {node} + node.right.Repr + if node.left != null then node.left.Repr else {};
+          node.Values := {node.value} + node.right.Values + if node.left != null then node.left.Values else {};
+          node.Priorities := {node.priority} + node.right.Priorities + if node.left != null then node.left.Priorities else {};
+          head := node;
+          if (node.right.priority > node.priority) {
+            head := RotateLeft(node);
+          }
+        }
+        assert node.Valid() && node.ValidHeap(); 
+      } 
     }
   }
 
@@ -48,82 +123,105 @@ class Treap {
     return ans;
   }
 
-  // Recursive search using nodes
-  method SearchNode(currRoot: TreapNode, value: int)
+  // // Recursive search using nodes
+  static method SearchNode(currRoot: TreapNode, val: int)
     returns (node: TreapNode?)
-    requires currRoot.Valid()
-    ensures if node != null then node.key == value else true
-    decreases currRoot.repr
+    requires currRoot.Valid() && currRoot.ValidHeap()
+    ensures if node != null then node.value == val else true
+    decreases currRoot.Repr
   {
-    if (currRoot.key == value) {
+    if (currRoot.value == val) {
       return currRoot;
     }
-    if (currRoot.key < value && currRoot.right != null) {
-      var ans := SearchNode(currRoot.right, value);
+    if (currRoot.value < val && currRoot.right != null) {
+      var ans := SearchNode(currRoot.right, val);
       return ans;
     }
-    if (currRoot.key > value && currRoot.left!= null) {
-      var ans := SearchNode(currRoot.left, value);
+    if (currRoot.value > val && currRoot.left!= null) {
+      var ans := SearchNode(currRoot.left, val);
       return ans;
     }
     return null;
   }
 
-  method InOrderTraversal() 
+  static method PreOrderTraversal(node: TreapNode?) 
+    requires node != null ==> node.Valid() && node.ValidHeap();
+    decreases if node != null then node.Repr else {}
   {
-    if (this.root != null) {
-      print this.root.key;
+    if (node == null) {
+      return;
+    } else {
+      print node.value, "|", node.priority, " ";
+      PreOrderTraversal(node.left);
+      PreOrderTraversal(node.right);
     }
   }
 
-  method RotateLeft(node: TreapNode)
-    returns (newNode: TreapNode)
-    requires node.right != null
-    requires node.Valid()
-    modifies node.repr
-    ensures old(node.repr) == newNode.repr // No change in reachability
-    ensures newNode.Valid() // Answer is valid
-    ensures newNode == old(node.right)
-    ensures newNode.right == old(newNode.right)
-    ensures newNode.left == node
-    ensures node.right == old(node.right.left)
-    ensures node.left == old(node.left)
+  static method RotateLeft(node: TreapNode) returns (newNode: TreapNode)
+    requires node.Valid() // The heap must NOT be valid
+    requires node.ValidRotateLeft()
+    modifies node.Repr
+    ensures newNode.Valid() && newNode.ValidHeap()
+    ensures node.Valid() && node.ValidHeap()
   {
     newNode := node.right;
     var tempNode := newNode.left;
-    newNode.left:= node;
-    node.repr := node.repr -newNode.repr;
+
     node.right:= tempNode;
-    if(tempNode != null) {
-      // need to add repr of tempNode into node to maintain validity
-      node.repr := node.repr + tempNode.repr + {tempNode};
-    }
-    newNode.repr := newNode.repr + node.repr;
+    node.Repr := node.Repr - newNode.Repr;
+    node.Repr := node.Repr + if node.right != null then node.right.Repr else {};
+
+    node.Values := node.Values - newNode.Values;
+    node.Values := node.Values + if node.right != null then node.right.Values else {};
+
+    node.Priorities := {node.priority} 
+                    + (if node.left != null then node.left.Priorities else {})
+                    + (if node.right != null then node.right.Priorities else {});
+
+    newNode.left:= node;
+    newNode.Repr := newNode.Repr - if tempNode != null then tempNode.Repr else {};
+    newNode.Repr := newNode.Repr + node.Repr;
+
+    newNode.Values := newNode.Values - if tempNode != null then tempNode.Values else {};
+    newNode.Values := newNode.Values + node.Values;
+
+    newNode.Priorities := {newNode.priority}
+                        + newNode.left.Priorities
+                        + (if newNode.right != null then newNode.right.Priorities else {});
     return newNode;
   }
 
-  method RotateRight(node: TreapNode)
-    returns (newNode: TreapNode)
-    requires node.left != null
-    requires node.Valid()
-    modifies node.repr
-    ensures newNode.Valid()
-    ensures newNode == old(node.left)
-    ensures newNode.left== old(newNode.left)
-    ensures newNode.right == node
-    ensures node.left == old(node.left.right)
-    ensures node.right== old(node.right)
+  static method RotateRight(node: TreapNode) returns (newNode: TreapNode)
+    requires node.Valid() // The heap must NOT be valid
+    requires node.ValidRotateRight()
+    modifies node.Repr
+    ensures newNode.Valid() && newNode.ValidHeap()
+    ensures node.Valid() && node.ValidHeap()
   {
     newNode := node.left;
     var tempNode := newNode.right;
-    newNode.right := node;
-    node.repr := node.repr - newNode.repr;
-    node.left := tempNode;
-    if(tempNode != null) {
-      // need to add repr of tempNode into node to maintain validity
-      node.repr := node.repr + tempNode.repr + {tempNode};
-    }
-    newNode.repr := newNode.repr + node.repr;
+
+    node.left:= tempNode;
+    node.Repr := node.Repr - newNode.Repr;
+    node.Repr := node.Repr + if node.left != null then node.left.Repr else {};
+
+    node.Values := node.Values - newNode.Values;
+    node.Values := node.Values + if node.left != null then node.left.Values else {};
+
+    node.Priorities := {node.priority} 
+                    + (if node.right != null then node.right.Priorities else {})
+                    + (if node.left != null then node.left.Priorities else {});
+
+    newNode.right:= node;
+    newNode.Repr := newNode.Repr - if tempNode != null then tempNode.Repr else {};
+    newNode.Repr := newNode.Repr + node.Repr;
+
+    newNode.Values := newNode.Values - if tempNode != null then tempNode.Values else {};
+    newNode.Values := newNode.Values + node.Values;
+
+    newNode.Priorities := {newNode.priority}
+                        + newNode.right.Priorities
+                        + (if newNode.left != null then newNode.left.Priorities else {});
     return newNode;
   }
 
@@ -135,10 +233,27 @@ class Treap {
 }
 
 // Used for testing
-method Main() {
+method Main()
+{
   var treap := new Treap();
+  // assert fresh(treap);
   treap.Insert(3);
-  treap.InOrderTraversal();
-  var result := treap.RandomNumberGenerator();
-  print (result);
+  if (treap.root != null) {
+    var check := Treap.InsertHelper(4,517, treap.root);
+    Treap.PreOrderTraversal(check);
+    if (check != null) {
+      var search := Treap.SearchNode(check, 4);
+      if (search != null) {
+        print "\n",search.value,"|",search.priority;
+      }
+    }
+    assert treap.root.Valid() && treap.root.ValidHeap();
+    assert check != null ==> check.Valid() && check.ValidHeap();
+    treap.Repr := {treap} + treap.root.Repr;
+    treap.Values := treap.Values + treap.root.Values;
+    treap.Priorities := treap.Priorities + treap.root.Priorities;
+    // assert treap.Valid();
+  }
+  // var result := treap.RandomNumberGenerator();
+  // print (result);
 }
