TreapNode.dfy
@@ -1,72 +1,117 @@
 class TreapNode {
-  const key: int
+  /** ---- Ghost Information ---- */
+  ghost var Values: set<int>
+  ghost var Priorities: set<int>
+  ghost var Repr: set<object>
+
+  ghost predicate Valid()
+    reads this, Repr
+    ensures Valid() ==> this in Repr
+  {
+    // This class must be inside set Repr
+    && this in Repr
+    // Validate the left side child
+    && (left != null ==>
+        && left in Repr
+        && left.Repr <= Repr
+        && this !in left.Repr
+        && left.Valid()
+        && forall x :: x in left.Values ==> x < value)
+    // Validate the right side child
+    && (right != null ==>
+        && right in Repr
+        && right.Repr <= Repr
+        && this !in right.Repr
+        && right.Valid()
+        && forall x :: x in right.Values ==> value < x)
+    && (left == null && right == null ==>
+        && Values == {value})
+    && (left != null && right == null ==>
+        && Values == left.Values + {value})
+    && (left == null && right != null ==>
+        && Values == right.Values + {value})
+    && (left != null && right != null ==> 
+        && left.Repr !! right.Repr
+        && Values == left.Values + {value} + right.Values)
+  }
+
+  ghost predicate ValidHeap()
+    reads this, Repr
+    requires Valid()
+    ensures ValidHeap() ==> this in Repr
+  {
+    && (left != null ==> 
+      && left.ValidHeap()
+      && forall y :: y in left.Priorities ==> y <= priority)
+    && (right != null ==> 
+      && right.ValidHeap()
+      && forall y :: y in right.Priorities ==> y <= priority)
+    && (left == null && right == null ==> Priorities == {priority})
+    && (left != null && right == null ==> Priorities == left.Priorities + {priority})
+    && (left == null && right != null ==> Priorities == right.Priorities + {priority})
+    && (left != null && right != null ==> Priorities == left.Priorities + {priority} + right.Priorities)
+
+  }
+
+  ghost predicate ValidRotateLeft()
+    reads this, Repr
+    requires Valid()
+  {
+    && (right != null
+      && priority < right.priority
+      && right.ValidHeap())
+    && (left != null ==> 
+      && (forall x :: x in left.Priorities ==> x <= priority)
+      && left.ValidHeap())
+    && (Priorities == {priority}
+      + (if left != null then left.Priorities else {})
+      + (if right != null then right.Priorities else {}))
+    && (right != null && right.left != null ==> 
+      (forall x :: x in right.left.Priorities ==> x <= priority))
+  }
+
+  ghost predicate ValidRotateRight()
+    reads this, Repr
+    requires Valid()  
+  {
+    && (left != null
+      && priority < left.priority
+      && left.ValidHeap())
+    && (right != null ==> 
+      && (forall x :: x in right.Priorities ==> x <= priority)
+      && right.ValidHeap())
+    && (Priorities == {priority}
+      + (if right != null then right.Priorities else {})
+      + (if left != null then left.Priorities else {}))
+    && (left != null && left.right != null ==> 
+      (forall x :: x in left.right.Priorities ==> x <= priority))
+  }
+
+  const value: int
   const priority: int
+
   var left: TreapNode?
   var right: TreapNode?
 
-  // Needed to ensure no cycles in between nodes
-  ghost var repr: set<TreapNode>
-
-  ghost predicate Valid()
-    reads this, repr
+  constructor (value:int, priority:int)
+    ensures Valid() && ValidHeap() && fresh(Repr)
+    ensures Values == {value}
+    ensures Priorities == {priority}
   {
-    && this in repr // node is reachable to itself
-    && ( left != null ==>
-         && left in repr
-         && this !in left.repr
-         && left.repr < repr
-         && left.Valid())
-    && ( right != null ==>
-         && right in repr
-         && this !in right.repr
-         && right.repr < repr
-         && right.Valid())
-    && ( // Extra check to ensure only one path between 2 nodes.
-       (right != null && left != null) ==>
-         ((forall x :: x in left.repr ==> x !in right.repr) &&
-                       (forall y :: y in right.repr ==> y !in left.repr)))
+    this.value := value;
+    this.priority := priority;
+    this.left := null;
+    this.right := null;
+
+    Repr := {this};
+    Values := {value};
+    Priorities := {priority};
   }
 
-  method insertNode(node: TreapNode?) 
-    requires this.Valid()
-    modifies this.repr
-    decreases this.repr
-  {
-    if (node == null) {return;}
-    if (node.key < this.key) {
-        // Go to the left
-        if (this.left == null) {
-            this.repr := this.repr + node.repr;
-            this.left := node;
-        } else {
-            this.left.insertNode(node);
-            // TODO: check priority
-        }
-    } else {
-      if (this.right == null) {
-            this.repr := this.repr + node.repr;
-            this.right := node;
-        } else {
-            this.right.insertNode(node);
-            // TODO: check priority
-        }
-    }
-  }
   predicate IsLeaf()
     reads this
   {
     && this.left == null
     && this.right == null
-  }
-
-  constructor (key:int, priority:int)
-    ensures Valid()
-    ensures repr == {this}
-  {
-    this.key := key;
-    this.priority := priority;
-    this.left := null;
-    this.right := null;
-    repr := {this};
   }
 }
